Nemonuri/TransitionSystemLike/SequentialHardwareCircuit.lean
@@ -21,25 +21,99 @@ namespace Nemonuri
 namespace SequentialHardwareCircuit
 
 /-- *n* input bits, *m* output bits, *k* registers -/
-structure Eval (n k: ℕ) where
+structure State (n k: ℕ) where
   inputs: Vector Bool n
   registers: Vector Bool k
   deriving DecidableEq
 
-namespace Eval
+
+namespace State
 
 
 def vectorEquiv (α: Type _) (n: ℕ) : Vector α n ≃ List.Vector α n where
   toFun v := ⟨v.toList, v.length_toList⟩
   invFun lv := ⟨lv.toArray, lv.property⟩
 
-def vectorProdEquiv (n k: ℕ) : Eval n k ≃ (List.Vector Bool n × List.Vector Bool k) where
+def vectorProdEquiv (n k: ℕ) : State n k ≃ (List.Vector Bool n × List.Vector Bool k) where
   toFun e := ⟨(vectorEquiv _ _) e.inputs, (vectorEquiv _ _) e.registers⟩
   invFun lv := ⟨(vectorEquiv _ _).symm lv.fst, (vectorEquiv _ _).symm lv.snd⟩
 
-instance toFintype {n k: ℕ} : Fintype (Eval n k) := Fintype.ofEquiv _ (vectorProdEquiv n k).symm
+instance toFintype {n k: ℕ} : Fintype (State n k) := Fintype.ofEquiv _ (vectorProdEquiv n k).symm
 
-end Eval
+#check Eq.refl
+#check HEq.subst
+
+/-
+theorem _root_.Vector.size_eq_of_heq {α: Type _} {n1 n2: ℕ} {v1: Vector α n1} {v2: Vector α n2} (req: v1 ≍ v2)
+  : n1 = n2 := by
+  let Spec (T: Type _) (x: T) : Prop := ∃(n: ℕ), ∃(h: T = Vector α n), ((cast h x).size = n1 ∧ n ≠ n2)
+  have lm2 : Spec _ v1 := by
+    simp [Spec]
+    exists n1
+    simp
+    exact lm1
+  have lm3 := req.subst lm2
+  subst Spec
+  simp at lm3
+  obtain ⟨n, ⟨lm3_1, lm3_2⟩, lm4⟩ := lm3
+  dsimp [Vector.size] at lm3_2
+-/
+
+
+
+
+
+/-
+  let Spec (T: Type _) (x: T) : Prop := ∃!(n: ℕ), ∃(h: T = Vector α n), ((cast h x).size = n1)
+  have lm1 : Spec _ v1 := by
+    simp [Spec, ExistsUnique]
+    exists n1
+    constructor
+    · exists rfl
+    · intro n lm1 lm2
+      dsimp [Vector.size] at lm2
+      exact lm2
+  have lm2 := req.subst lm1
+  subst Spec
+  simp [ExistsUnique] at lm2
+  obtain ⟨n, ⟨lm2_1, lm2_2⟩, lm3⟩ := lm2
+  have lm4 := lm3 n2 rfl
+  dsimp [Vector.size] at lm4
+  have lm5 := type_eq_of_heq req
+  have lm6 := lm3 n1 lm5.symm
+  dsimp [Vector.size] at lm6
+  simp at lm6
+-/
+  --simp [ExistsUnique] at lm1
+
+
+/-
+  have lm1 := Eq.refl v2.size
+  conv at lm1 => rhs; dsimp [Vector.size]
+  have lm2 : v1.size = n2 := @req.subst
+-/
+
+  --by_contra lm1
+  --obtain ⟨lm4, lm5⟩ := heq_iff_exists_cast_eq.mp req.symm
+  --have lm3 := congrArg (Vector.size) lm2
+  --dsimp [Vector.size] at lm3
+  --rewrite [Vector.ext_iff] at lm2
+  --rewrite [heq_iff_exists_cast_eq] at req
+
+  --have lm1 := type_eq_of_heq req
+  --have := req.
+  --have := Vector.ext
+/-
+  rcases v1 with ⟨⟨l1⟩, lm1⟩
+  rcases v2 with ⟨⟨l2⟩, lm2⟩
+  revert lm1 lm2
+  simp
+  intro lm1 lm2 req
+-/
+  --have lm3 := type_eq_of_heq req
+
+
+end State
 
 
 inductive Act where
@@ -47,7 +121,7 @@ inductive Act where
   deriving DecidableEq, Fintype
 
 
-inductive AP (n m k: ℕ) where
+inductive AtomicProp (n m k: ℕ) where
   | inputs (i: Fin n)
   | outputs (i: Fin m)
   | registers (i: Fin k)
@@ -60,7 +134,7 @@ inductive AP (n m k: ℕ) where
   deriving DecidableEq
 -/
 
-namespace AP
+namespace AtomicProp
 
 /-
 def vectorEvalProdEquiv (n m k: ℕ) : AP n m k ≃ (List.Vector Bool m × Eval n k) where
@@ -70,7 +144,7 @@ def vectorEvalProdEquiv (n m k: ℕ) : AP n m k ≃ (List.Vector Bool m × Eval 
 instance toFintype {n m k: ℕ} : Fintype (AP n m k) := Fintype.ofEquiv _ (vectorEvalProdEquiv n m k).symm
 -/
 
-theorem not_all_zero (ap: AP 0 0 0) : False := by
+theorem not_all_zero (ap: AtomicProp 0 0 0) : False := by
   cases ap <;> (
     rename_i i
     rcases i with ⟨i, lm1⟩
@@ -78,7 +152,7 @@ theorem not_all_zero (ap: AP 0 0 0) : False := by
 
 variable {n m k: ℕ}
 
-theorem any_ne_zero (ap: AP n m k) : (n ≠ 0) ∨ (m ≠ 0) ∨ (k ≠ 0) := by
+theorem any_ne_zero (ap: AtomicProp n m k) : (n ≠ 0) ∨ (m ≠ 0) ∨ (k ≠ 0) := by
   by_contra lm1
   simp at lm1
   rcases lm1 with ⟨lm1_1, lm1_2, lm1_3⟩
@@ -87,7 +161,7 @@ theorem any_ne_zero (ap: AP n m k) : (n ≠ 0) ∨ (m ≠ 0) ∨ (k ≠ 0) := by
   subst lm1_3
   exact ap.not_all_zero
 
-theorem nonempty_iff_any_ne_zero : (Nonempty (AP n m k)) ↔ ((n ≠ 0) ∨ (m ≠ 0) ∨ (k ≠ 0)) := by
+theorem nonempty_iff_any_ne_zero : (Nonempty (AtomicProp n m k)) ↔ ((n ≠ 0) ∨ (m ≠ 0) ∨ (k ≠ 0)) := by
   constructor
   · rintro ⟨ap⟩
     exact ap.any_ne_zero
@@ -99,22 +173,22 @@ theorem nonempty_iff_any_ne_zero : (Nonempty (AP n m k)) ↔ ((n ≠ 0) ∨ (m �
       · exact .intro (.outputs (.mk 0 lm1))
       · exact .intro (.registers (.mk 0 lm1))
 
-def combineBPred (fi: (Fin n) → Bool) (fo: (Fin m) → Bool) (fr: (Fin k) → Bool) (ap: AP n m k) : Bool :=
+def combineBPred (fi: (Fin n) → Bool) (fo: (Fin m) → Bool) (fr: (Fin k) → Bool) (ap: AtomicProp n m k) : Bool :=
   match ap with
   | .inputs i => fi i
   | .registers i => fr i
   | .outputs i => fo i
 
-end AP
+end AtomicProp
 
 
-def labeling {n m k: ℕ} (sw: (Eval n k) → (Fin m) → Bool) (ev: Eval n k) (ap: AP n m k) : Bool :=
+def labeling {n m k: ℕ} (sw: (State n k) → (Fin m) → Bool) (ev: State n k) (ap: AtomicProp n m k) : Bool :=
   match ap with
   | .inputs i => ev.inputs.get i
   | .registers i => ev.registers.get i
   | .outputs i => sw ev i
 
-namespace Eval
+namespace State
 
 /-
 def ofFn {n m k: ℕ} (fn: (AP n m k) → Bool) : Eval n k :=
@@ -123,7 +197,7 @@ def ofFn {n m k: ℕ} (fn: (AP n m k) → Bool) : Eval n k :=
   Eval.mk (inputs (by simp)) (registers (by simp))
 -/
 
-def ofFn {n k: ℕ} (fi: (Fin n) → Bool) (fr: (Fin k) → Bool) : Eval n k := Eval.mk (.ofFn fi) (.ofFn fr)
+def ofFn {n k: ℕ} (fi: (Fin n) → Bool) (fr: (Fin k) → Bool) : State n k := State.mk (.ofFn fi) (.ofFn fr)
 
 /-
 theorem ofFn_labeling {n m k: ℕ} (sw: (Eval n k) → (Fin m) → Bool) (fi: (Fin n) → Bool) (fr: (Fin k) → Bool)
@@ -140,45 +214,165 @@ theorem ofFn_labeling {n m k: ℕ} (sw: (Eval n k) → (Fin m) → Bool) (fi: (F
     dsimp
 -/
 
-def ofAPBoolPred {n m k: ℕ} (bpred: AP n m k → Bool) : Eval n k :=
-  let fi (i: Fin n) := bpred (AP.inputs i)
-  let fr (i: Fin k) := bpred (AP.registers i)
-  Eval.ofFn fi fr
+def ofAPBoolPred {n m k: ℕ} (bpred: AtomicProp n m k → Bool) : State n k :=
+  let fi (i: Fin n) := bpred (AtomicProp.inputs i)
+  let fr (i: Fin k) := bpred (AtomicProp.registers i)
+  State.ofFn fi fr
 
-end Eval
+end State
+
+structure Indexed (n m k: ℕ) where
+  initialRegisters: Vector Bool k
+  outputFn : (State n k) → (Fin m) → Bool
+  registerFn : (State n k) → (Fin k) → Bool
+
+namespace Indexed
+
+variable {n m k: ℕ}
+
+@[mk_iff]
+inductive Transition (shcI: Indexed n m k) : (State n k) → Act → (State n k) → Prop where
+  | intro (s1: State n k) (s2i: Vector Bool n) : Transition shcI s1 .τ (State.mk s2i (Vector.ofFn (shcI.registerFn s1)))
+
+@[reducible]
+def toTransitionSystem (shcI: Indexed n m k) : TransitionSystem where
+  S := State n k
+  Act := Act
+  I := { s: State n k | s.registers = shcI.initialRegisters }
+  AP := AtomicProp n m k
+  L := labeling shcI.outputFn
+  tr := shcI.Transition
+
+theorem toTransitionSystem_injective : Function.Injective (@toTransitionSystem n m k) := by
+  rintro ⟨ir1, of1, rf1⟩ ⟨ir2, of2, rf2⟩
+  simp [toTransitionSystem]
+  intro lm1 lm2 lm3
+  refine ⟨?_, ?_, ?_⟩
+  · clear lm1 lm3
+    simp [Set.ext_iff] at lm2
+    have lm2_1 := lm2 ⟨default, ir1⟩
+    simp at lm2_1
+    exact lm2_1
+  · clear lm1 lm2
+    simp only [funext_iff]
+    intro s oi
+    simp only [funext_iff] at lm3
+    specialize lm3 s (AtomicProp.outputs oi)
+    dsimp [labeling] at lm3
+    exact lm3
+  · clear lm2 lm3
+    simp only [funext_iff]
+    intro s ri
+    simp only [funext_iff] at lm1
+    specialize lm1 s .τ (State.mk default (Vector.ofFn (rf1 s)))
+    simp [transition_iff] at lm1
+    rewrite [Vector.ext_iff] at lm1
+    simp at lm1
+    specialize lm1 ri.val ri.isLt
+    simp at lm1
+    exact lm1
+
+end Indexed
 
 end SequentialHardwareCircuit
 
+
 open SequentialHardwareCircuit in
-structure SequentialHardwareCircuit (n m k: ℕ) where
-  initialRegisters: Vector Bool k
-  --apFilter : (AP n m k) → Bool
-  outputFn : (Eval n k) → (Fin m) → Bool
-  registerFn : (Eval n k) → (Fin k) → Bool
+structure SequentialHardwareCircuit where --(n m k: ℕ)
+  inputLength : ℕ
+  registerLength : ℕ
+  outputLength : ℕ
+  indexed : Indexed inputLength registerLength outputLength
+  --initialRegisters: Vector Bool registerLength
+  --outputFn : (State inputLength registerLength) → (Fin outputLength) → Bool
+  --registerFn : (State inputLength registerLength) → (Fin registerLength) → Bool
+
 
 namespace SequentialHardwareCircuit
 
+#check type_eq_of_heq
+
+@[reducible]
+def toTransitionSystem (shc: SequentialHardwareCircuit) : TransitionSystem := shc.indexed.toTransitionSystem
+
+
+/-
+theorem toTransitionSystem_injective : Function.Injective (toTransitionSystem) := by
+  intro shc1 shc2 lm1
+  dsimp [toTransitionSystem] at lm1
+  dsimp [Indexed.toTransitionSystem] at lm1
+  simp at lm1
+  revert lm1
+  simp
+  intro lm1 lm2 lm3 lm4 lm5
+  have lm6 := type_eq_of_heq lm2
+-/
+  --have lm2 := Indexed.toTransitionSystem_injective.eq_iff.mp lm1
+  --have lm2 := fun n m k => @Indexed.toTransitionSystem_injective n m k
+  --dsimp [Function.Injective] at lm2
+  --dsimp [Indexed.toTransitionSystem] at lm1
+/-
+  rcases shc1 with ⟨n1, m1, k1, shcI1⟩
+  rcases shc2 with ⟨n2, m2, k2, shcI2⟩
+  simp at lm1 ⊢
+-/
+
+
 --def toLabeling {n m k: ℕ} (shc: SequentialHardwareCircuit n m k) (s: Eval n k) (ap: Subtype (shc.apFilter · = .true)) : Bool := labeling shc.outputFn s ap.val
 
+/-
 @[mk_iff]
-inductive Transition {n m k: ℕ} (shc: SequentialHardwareCircuit n m k) : (Eval n k) → Act → (Eval n k) → Prop where
-  | intro (s1: Eval n k) (s2i: Vector Bool n) : Transition shc s1 .τ (Eval.mk s2i (Vector.ofFn (shc.registerFn s1)))
+inductive Transition (shc: SequentialHardwareCircuit) : (State shc.inputLength shc.registerLength) → Act → (State shc.inputLength shc.registerLength) → Prop where
+  | intro (s1: State shc.inputLength shc.registerLength) (s2i: Vector Bool shc.inputLength) : Transition shc s1 .τ (State.mk s2i (Vector.ofFn (shc.registerFn s1)))
 
 
 @[reducible]
-def toTransitionSystem {n m k: ℕ} (shc: SequentialHardwareCircuit n m k) : TransitionSystem where
-  S := Eval n k
+def toTransitionSystem (shc: SequentialHardwareCircuit) : TransitionSystem where
+  S := State shc.inputLength shc.registerLength
   Act := Act
-  I := { e: Eval n k | e.registers = shc.initialRegisters }
-  AP := AP n m k
+  I := { s: State shc.inputLength shc.registerLength | s.registers = shc.initialRegisters }
+  AP := AtomicProp shc.inputLength shc.outputLength shc.registerLength
   L := labeling shc.outputFn
   tr := shc.Transition
 
 
-theorem toTransitionSystem_injective {n m k: ℕ} : Function.Injective (@toTransitionSystem n m k) := by
-  rintro ⟨ir1, of1, rf1⟩ ⟨ir2, of2, rf2⟩
+theorem toTransitionSystem_injective : Function.Injective (toTransitionSystem) := by
+  --rintro ⟨n1, m1, k1, ir1, of1, rf1⟩ ⟨n2, m2, k2, ir2, of2, rf2⟩
+  intro shc1 shc2
   simp [toTransitionSystem]
-  intro lm1 lm2 lm3
+  intro lm1 lm2 lm3 lm4 lm5
+  rewrite [heq_iff_exists_cast_eq] at lm3
+  rcases lm3 with ⟨lm6, lm3⟩
+  rewrite [Set.ext_iff] at lm3
+  simp at lm3
+  let st1 : State shc2.inputLength shc2.registerLength := .mk default shc2.initialRegisters
+  specialize lm3 st1
+  subst st1
+  simp at lm3
+  dsimp [cast] at lm3
+/-
+  rewrite [heq_iff_exists_cast_eq] at lm2
+  rcases lm2 with ⟨lm6, lm2⟩
+  simp only [funext_iff] at lm2
+  simp at lm2
+-/
+/-
+
+  rcases ir1 with ⟨⟨ir1_l⟩, ir1_s⟩
+  rcases ir2 with ⟨⟨ir2_l⟩, ir2_s⟩
+  revert lm2 lm3 ir1_s ir2_s
+  simp
+  intro ir1_s ir2_s lm2 lm3
+  unfold labeling at lm5
+-/
+
+
+  --rintro ⟨n1, m1, k1, ir1, of1, rf1⟩ ⟨n2, m2, k2, ir2, of2, rf2⟩
+
+  --intro lm1 lm2 lm3 lm4 lm5
+/-
+
+
   refine ⟨?_, ?_, ?_⟩
   · clear lm1 lm3
     simp [Set.ext_iff] at lm2
@@ -203,8 +397,9 @@ theorem toTransitionSystem_injective {n m k: ℕ} : Function.Injective (@toTrans
     specialize lm1 ri.val ri.isLt
     simp at lm1
     exact lm1
+-/
 
-
+@[simp]
 instance {n m k: ℕ} : TransitionSystemLike (SequentialHardwareCircuit n m k) where
   coe := toTransitionSystem
   coe_injective := toTransitionSystem_injective
@@ -225,17 +420,27 @@ instance : ConcreteFinite (shc: TransitionSystem) :=
 --instance : Fintype ((shc: TransitionSystem).AP) := inferInstance
 
 /-
-set_option trace.Meta.synthInstance true in
+--set_option trace.Meta.synthInstance true in
 open PropositionalLogics in
 theorem labeling_valid (s: Eval n k)
   : let ts := (shc: TransitionSystem)
-    let : EvalLike (Quotient ts.toLabelingSetoid) (AP n m k) := inferInstanceAs (EvalLike (Quotient ts.toLabelingSetoid) ts.AP)
+    --let : EvalLike (Quotient ts.toLabelingSetoid) (AP n m k) := inferInstanceAs (EvalLike (Quotient ts.toLabelingSetoid) ts.AP)
     𝐿{ts}⸨s⸩ = (
       (Finset.image AP.inputs { xᵢ: Fin n | ts.labeling s (.inputs xᵢ) = .true }) ∪
       (Finset.image AP.registers { rᵢ: Fin k | ts.labeling s (.registers rᵢ) = .true }) ∪
-      (Finset.image AP.outputs { yᵢ: Fin m | ⟦s⟧{ts} ⊨ₚ ((.atom (AP.outputs yᵢ : AP n m k))) })
+      (Finset.image AP.outputs { yᵢ: Fin m | shc.outputFn s yᵢ = .true  })
     )
+  := by
+  extract_lets ts
+  simp [Finset.ext_iff]
+  dsimp [evalStateToFinset, TransitionSystem.labeling]
+  intro ap
+  subst ts
+  dsimp at ap ⊢
+  --revert ap
+  --simp --[TransitionSystemLike.coe]
 -/
+
 end TransitionSystem
 /-
 theorem toTransitionSystem_labeling_injective {n m k: ℕ} {shc: SequentialHardwareCircuit n m k} [NeZero m] : Function.Injective ((shc: TransitionSystem).L) := by
@@ -263,7 +468,7 @@ instance {n m k: ℕ} {shc: SequentialHardwareCircuit n m k} : Eval.EvalLike (sh
     · dsimp [labeling] at lm1
     --have := AP.outputs default
 -/
-
+-/
 end SequentialHardwareCircuit
 
 end Nemonuri
